\begin{eqnarray*}
D
&=&
\frac{
1
}{
3
}
\lambda
\overline{c}
\\ &=&
\frac{
1
}{
3
}
\cdot
\frac{
KT
}{
\sqrt{
2
}
\rho
P
}
\cdot
\sqrt{
\frac{
8KT
}{
\pi
m
}
}
\\ &=&
\frac{
1
}{
3
}
\cdot
\sqrt{
\frac{
{
(
\uni[1.38 \times 10^{-23}]{J.K^{-1}}
\cdot
\uni[298]{K}
)
}^{
3
}
}{
2
\cdot
\pi
\cdot
\uni[39.95]{
g.mol^{-1}
}
}
}
\cdot
\frac{
1
}{
\uni[
0.36 \times
10^{-18}
]{
m^2
}
\cdot
\uni[1]{
atm
}
}
\\ &=&
\uni[1.541 \times 10^{-4}]{
J^{-\frac{3}{2}}.m^{-2}.atm^{-1}
}
\\ &=&
\uni[1.53 \times 10^{-19}]{
m.s^{-1}
}
\label{}
\end{eqnarray*}